Movement of some of the more useful list functions (FOLDL,FOLDR, EXISTS,MEM) from rich_list to list. Also, proved congruence theorems for higher-order functions (supports bossLib.Define).

src/list/src/listScript.sml
@@ -4,8 +4,8 @@
 (*                 type is defined and the following "axiomatization" is *)
 (*                 proven from the definition of the type:               *)
 (*                                                                       *)
-(*                    |- !x f. ?!fn. (fn NIL = x) /\                     *)
-(*                             (!h t. fn (CONS h t) = f (fn t) h t) *)
+(*                    |- !x f. ?!fn. (fn [] = x) /\                     *)
+(*                             (!h t. fn (h::t) = f (fn t) h t)      *)
 (*                                                                       *)
 (*                 Translated from hol88.                                *)
 (*                                                                       *)
@@ -20,10 +20,11 @@
 structure listScript =
 struct
 
-(*---------------------------------------------------------------------------
- * Bind ancestor theory structures. The parents of list are "arithmetic" and
- * "pair".
+(*---------------------------------------------------------------------------*
+ * Require ancestor theory structures to be present. The parents of list     *
+ * are "arithmetic" and "pair".                                              *
  *---------------------------------------------------------------------------*)
+
 local open arithmeticTheory pairTheory in end;
 
 val _ = Rewrite.add_implicit_rewrites pairTheory.pair_rws;
@@ -32,6 +33,7 @@ val _ = Rewrite.add_implicit_rewrites pairTheory.pair_rws;
 (*---------------------------------------------------------------------------
  * Open structures used in the body.
  *---------------------------------------------------------------------------*)
+
 open HolKernel Parse basicHol90Lib Num_conv ;
 infix THEN ORELSE THENL THENC ORELSEC  |->;
 
@@ -62,6 +64,7 @@ val LESS_MONO_EQ  = arithmeticTheory.LESS_MONO_EQ;
 val ADD_CLAUSES   = arithmeticTheory.ADD_CLAUSES;
 val LESS_MONO_EQ  = arithmeticTheory.LESS_MONO_EQ;
 val ADD_EQ_0      = arithmeticTheory.ADD_EQ_0;
+val ONE           = arithmeticTheory.ONE;
 
 val PAIR_EQ = pairTheory.PAIR_EQ;
 
@@ -114,6 +117,7 @@ new_definition("CONS_DEF",
 
 val _ = add_listform {separator = ";", leftdelim = "[", rightdelim = "]",
                       cons = "CONS", nilstr = "NIL"};
+
 val _ = add_rule {term_name = "CONS", fixity = Infixr 300,
                   pp_elements = [TOK "::"],
                   paren_style = OnlyIfNecessary,
@@ -137,11 +141,9 @@ val lemma1 =
 	       (\b m g. f (b (\i.g(i+1))) (g 0) (ABS_list((\i.g(i+1)),m))))
      (SND p)
      (FST p)`--)
-   THEN
-   CONV_TAC (DEPTH_CONV (BETA_CONV ORELSEC num_CONV)) THEN
-   REWRITE_TAC [PRIM_REC_THM, ADD_CLAUSES] THEN
-   CONV_TAC (DEPTH_CONV BETA_CONV) THEN
-   REWRITE_TAC[]);
+   THEN CONV_TAC (DEPTH_CONV BETA_CONV)
+   THEN REWRITE_TAC [PRIM_REC_THM, ADD_CLAUSES, ONE]
+   THEN CONV_TAC (DEPTH_CONV BETA_CONV) THEN REWRITE_TAC[]);
 
 val NIL_lemma =
     TAC_PROOF(([], --`REP_list NIL = ((\n:num.@x:'a.T), 0)`--),
@@ -156,7 +158,7 @@ val REP_lemma =
 	      REFL_TAC);
 
 val CONS_lemma = TAC_PROOF(([],
-   --`REP_list (CONS (h:'a) t) =
+   --`REP_list ((h:'a):: t) =
      ((\m.((m=0)=>h|FST(REP_list t)(PRE m))),SUC(SND(REP_list t)))`--),
    REWRITE_TAC [CONS_DEF, (SYM(SPEC_ALL R_A)), IS_list_REP] THEN
    EXISTS_TAC (--`\n.((n=0) => (h:'a) | (FST(REP_list t)(PRE n)))`--) THEN
@@ -174,16 +176,16 @@ val CONS_lemma = TAC_PROOF(([],
    REWRITE_TAC [NOT_LESS, (SYM(SPEC_ALL LESS_EQ))] THEN
    CONV_TAC (DEPTH_CONV BETA_CONV) THEN
    DISCH_THEN ((STRIP_THM_THEN SUBST1_TAC) o MATCH_MP LESS_ADD_1) THEN
-   REWRITE_TAC [num_CONV (--`1`--), PRE, ADD_CLAUSES, NOT_SUC] THEN
+   REWRITE_TAC [arithmeticTheory.ONE, PRE, ADD_CLAUSES, NOT_SUC] THEN
    REWRITE_TAC[REWRITE_RULE[SYM(SPEC_ALL NOT_LESS)] LESS_EQ_ADD]);
 
 val exists_lemma = TAC_PROOF(([],
  --`!x:'b. !(f :'b->'a->'a list->'b).
     ?fn1:'a list->'b.
        (fn1 NIL = x) /\
-       (!h t. fn1 (CONS h t) = f (fn1 t) h t)`--),
+       (!h t. fn1 (h::t) = f (fn1 t) h t)`--),
     REPEAT STRIP_TAC THEN
-    STRIP_ASSUME_TAC (REWRITE_RULE [num_CONV (--`1`--), ADD_CLAUSES]
+    STRIP_ASSUME_TAC (REWRITE_RULE [ONE, ADD_CLAUSES]
 		   (SPECL[--`x:'b`--, --`f:'b->'a->'a list->'b`--]
                          lemma1)) THEN
     EXISTS_TAC (--`\(x:('a)list).(fn1 (REP_list x):'b)`--) THEN
@@ -231,8 +233,8 @@ val list_Axiom = store_thm("list_Axiom",
  --`!x:'b.
     !f:'b -> 'a -> 'a list -> 'b.
     ?!(fn1: 'a list -> 'b).
-        (fn1 NIL = x) /\
-        (!h t. fn1 (CONS h t) = f (fn1 t) h t)`--,
+        (fn1 [] = x) /\
+        (!h t. fn1 (h::t) = f (fn1 t) h t)`--,
     PURE_REWRITE_TAC [boolTheory.EXISTS_UNIQUE_DEF] THEN
     CONV_TAC (REDEPTH_CONV BETA_CONV) THEN
     REWRITE_TAC [exists_lemma] THEN
@@ -254,77 +256,117 @@ val list_Axiom = store_thm("list_Axiom",
                 (SPEC (--`\n.f'(SUC n):'a`--))) THEN
      ASM_REWRITE_TAC [cons_lemma]]);
 
+
+(*---------------------------------------------------------------------------
+     Now some definitions.
+ ---------------------------------------------------------------------------*)
+
 val NULL_DEF = new_recursive_definition
       {name = "NULL_DEF",
        fixity = Prefix,
        rec_axiom = list_Axiom,
-       def = --`(NULL (NIL:'a list) = T) /\
-                (NULL (CONS (h:'a) t) = F)`--};
+       def = --`(NULL []     = T) /\
+                (NULL (h::t) = F)`--};
 
 val HD = new_recursive_definition
       {name = "HD",
        fixity = Prefix,
        rec_axiom = list_Axiom,
-       def = --`HD (CONS (h:'a) t) = h`--};
+       def = --`HD (h::t) = h`--};
 
 val TL = new_recursive_definition
       {name = "TL",
        fixity = Prefix,
        rec_axiom = list_Axiom,
-       def = --`TL (CONS (h:'a) t) = t`--};
+       def = --`TL (h::t) = t`--};
 
 val SUM = new_recursive_definition
       {name = "SUM",
        fixity = Prefix,
        rec_axiom =  list_Axiom,
-       def = --`(SUM NIL = 0) /\
-                (!h t. SUM (CONS h t) = h + (SUM t))`--};
+       def = --`(SUM [] = 0) /\
+          (!h t. SUM (h::t) = h + SUM t)`--};
 
 val APPEND = new_recursive_definition
       {name = "APPEND",
        fixity = Prefix,
        rec_axiom = list_Axiom,
-       def = --`(!l:'a list. APPEND NIL l = l) /\
-                (!l1 l2 h. APPEND (CONS h l1) l2 = CONS h (APPEND l1 l2))`--};
+       def = --`(!l:'a list. APPEND [] l = l) /\
+                  (!l1 l2 h. APPEND (h::l1) l2 = h::APPEND l1 l2)`--};
 
 val FLAT = new_recursive_definition
       {name = "FLAT",
        fixity = Prefix,
        rec_axiom = list_Axiom,
-       def = --`(FLAT NIL = (NIL:'a list)) /\
-                (!h t. FLAT (CONS h t) = APPEND h (FLAT t))`--};
+       def = --`(FLAT []     = []) /\
+          (!h t. FLAT (h::t) = APPEND h (FLAT t))`--};
 
 val LENGTH = new_recursive_definition
       {name = "LENGTH",
        fixity = Prefix,
        rec_axiom = list_Axiom,
-       def = --`(LENGTH NIL = 0) /\
-                (!(h:'a). !t. LENGTH (CONS h t) = SUC (LENGTH t))`--};
+       def = --`(LENGTH []     = 0) /\
+     (!(h:'a) t. LENGTH (h::t) = SUC (LENGTH t))`--};
 
 val MAP = new_recursive_definition
       {name = "MAP",
        fixity = Prefix,
        rec_axiom = list_Axiom,
-       def = --`(!f. MAP f NIL = NIL) /\
-                (!f h t. MAP f (CONS (h:'a) t) = CONS (f h:'b) (MAP f t))`--};
+       def = --`(!f:'a->'b. MAP f [] = []) /\
+                   (!f h t. MAP f (h::t) = f h::MAP f t)`--};
 
-(*---------------------------------------------------------------------------*
- * Added to support TFL -- kxs, June 1997                                    *
- *---------------------------------------------------------------------------*)
-val list_case_def = new_recursive_definition
-      {name = "list_case_def",
+val MEM = new_recursive_definition
+      {name = "MEM",
        fixity = Prefix,
        rec_axiom = list_Axiom,
-       def = --`(!b f. list_case b f NIL = (b:'b)) /\
-            (!b f h t. list_case b f (CONS (h:'a) t) = f h t)`--};
+       def = --`(!x. MEM x [] = F) /\
+            (!x h t. MEM x (h::t) = (x=h) \/ MEM x t)`--};
 
-(*---------------------------------------------------------------------------*
- * Added to support TFL -- kxs, Sept 1998                                    *
- *---------------------------------------------------------------------------*)
-val list_size_def = new_recursive_definition
-    {def = Term`(list_size f [] = 0) /\
-                (list_size f (CONS h t) = 1 + f h + list_size f t)`,
-     fixity = Prefix, name = "list_size_def", rec_axiom = list_Axiom};
+val FILTER = new_recursive_definition
+      {name = "FILTER",
+       fixity = Prefix,
+       rec_axiom = list_Axiom,
+       def = --`(!P. FILTER P [] = []) /\
+             (!(P:'a->bool) h t. 
+                    FILTER P (h::t) = 
+                         if P h then (h::FILTER P t) else FILTER P t)`--};
+
+
+val FOLDR = new_recursive_definition
+      {name = "FOLDR",
+       fixity = Prefix,
+       rec_axiom = list_Axiom,
+       def = --`(!f e. FOLDR (f:'a->'b->'b) e [] = e) /\
+            (!f e x l. FOLDR f e (x::l) = f x (FOLDR f e l))`--};
+
+val FOLDL = new_recursive_definition
+      {name = "FOLDL",
+       fixity = Prefix,
+       rec_axiom = list_Axiom,
+       def = --`(!f e. FOLDL (f:'b->'a->'b) e [] = e) /\
+            (!f e x l. FOLDL f e (x::l) = FOLDL f (f e x) l)`--};
+
+val EVERY_DEF = new_recursive_definition
+      {name = "EVERY_DEF",
+       fixity = Prefix,
+       rec_axiom = list_Axiom,
+       def = --`(!P:'a->bool. EVERY P [] = T)  /\
+                (!P h t. EVERY P (h::t) = P h /\ EVERY P t)`--};
+
+val EXISTS_DEF = new_recursive_definition
+      {name = "EXISTS_DEF",
+       fixity = Prefix,
+       rec_axiom = list_Axiom,
+       def = --`(!P:'a->bool. EXISTS P [] = F)  
+            /\  (!P h t.      EXISTS P (h::t) = P h \/ EXISTS P t)`--};
+
+val EL = new_recursive_definition
+      {name = "EL",
+       fixity = Prefix,
+       rec_axiom = num_Axiom,
+       def = --`(!l. EL 0 l = (HD l:'a)) /\
+                (!l:'a list. !n. EL (SUC n) l = EL n (TL l))`--};
+
 
 (* ---------------------------------------------------------------------*)
 (* Definition of a function 						*)
@@ -335,7 +377,7 @@ val list_size_def = new_recursive_definition
 (* 									*)
 (* |- (!f. MAP2 f[][] = []) /\						*)
 (*   (!f h1 t1 h2 t2.							*)
-(*      MAP2 f(CONS h1 t1)(CONS h2 t2) = CONS(f h1 h2)(MAP2 f t1 t2))	*)
+(*      MAP2 f(h1::t1)(h2::t2) = CONS(f h1 h2)(MAP2 f t1 t2))	*)
 (* 									*)
 (* [TFM 92.04.21]							*)
 (* ---------------------------------------------------------------------*)
@@ -345,10 +387,10 @@ val MAP2 =
      (--`?fn.
          (!f:'a -> 'b -> 'c. fn f [] [] = []) /\
          (!f h1 t1 h2 t2.
-           fn f (CONS h1 t1) (CONS h2 t2) = CONS (f h1 h2) (fn f t1 t2))`--,
+           fn f (h1::t1) (h2::t2) = f h1 h2::fn f t1 t2)`--,
       let val th = prove_rec_fn_exists list_Axiom
            (--`(fn (f:'a -> 'b -> 'c) [] l = []) /\
-               (fn f (CONS h t) l = CONS (f h (HD l)) (fn f t (TL l)))`--)
+               (fn f (h::t) l = CONS (f h (HD l)) (fn f t (TL l)))`--)
       in
       STRIP_ASSUME_TAC th THEN
       EXISTS_TAC (--`fn:('a -> 'b -> 'c) -> 'a list -> 'b list -> 'c list`--)
@@ -359,19 +401,25 @@ val MAP2 =
                     consts = [{const_name="MAP2", fixity=Prefix}]}
   end
 
-val EL = new_recursive_definition
-      {name = "EL",
-       fixity = Prefix,
-       rec_axiom = num_Axiom,
-       def = --`(!l. EL 0 l = (HD l:'a)) /\
-                (!l:'a list. !n. EL (SUC n) l = EL n (TL l))`--};
+(*---------------------------------------------------------------------------*
+ * Added to support TFL -- kxs, June 1997                                    *
+ *---------------------------------------------------------------------------*)
 
-val EVERY_DEF = new_recursive_definition
-      {name = "EVERY_DEF",
+val list_case_def = new_recursive_definition
+      {name = "list_case_def",
        fixity = Prefix,
        rec_axiom = list_Axiom,
-       def = --`(!P:'a->bool. EVERY P NIL = T)  /\
-                (!P h t. EVERY P (CONS h t) = (P h /\ EVERY P t))`--};
+       def = --`(!b f. list_case b f [] = (b:'b)) /\
+            (!b f h t. list_case b f (h:'a :: t) = f h t)`--};
+
+(*---------------------------------------------------------------------------*
+ * Added to support TFL -- kxs, Sept 1998                                    *
+ *---------------------------------------------------------------------------*)
+
+val list_size_def = new_recursive_definition
+    {def = Term`(list_size f [] = 0) /\
+                (list_size f (h::t) = 1 + f h + list_size f t)`,
+     fixity = Prefix, name = "list_size_def", rec_axiom = list_Axiom};
 
 
 (* ---------------------------------------------------------------------*)
@@ -379,20 +427,28 @@ val EVERY_DEF = new_recursive_definition
 (* ---------------------------------------------------------------------*)
 
 val NULL = store_thm ("NULL",
- --`NULL (NIL :'a list) /\ (!h t. ~NULL(CONS (h:'a) t))`--,
+ --`NULL ([] :'a list) /\ (!h t. ~NULL(CONS (h:'a) t))`--,
    REWRITE_TAC [NULL_DEF]);
 
-(* List induction							*)
-(* |- P NIL /\ (!t. P t ==> !h. P(CONS h t)) ==> (!x.P x) 		*)
+(*---------------------------------------------------------------------------*)
+(* List induction                                                            *)
+(* |- P [] /\ (!t. P t ==> !h. P(h::t)) ==> (!x.P x)                         *)
+(*---------------------------------------------------------------------------*)
+
 val list_INDUCT = save_thm("list_INDUCT",prove_induction_thm list_Axiom);
 
-(* Create a tactic.							*)
 val LIST_INDUCT_TAC = INDUCT_THEN list_INDUCT ASSUME_TAC;
 
-(* Cases theorem: |- !l. (l = []) \/ (?t h. l = CONS h t)		*)
+(*---------------------------------------------------------------------------*)
+(* Cases theorem: |- !l. (l = []) \/ (?t h. l = h::t)                        *)
+(*---------------------------------------------------------------------------*)
+
 val list_CASES = save_thm("list_CASES", prove_cases_thm list_INDUCT);
 
-(* CONS11:  |- !h t h' t'. (CONS h t = CONS h' t') = (h = h') /\ (t = t') *)
+(*---------------------------------------------------------------------------*)
+(* CONS11:  |- !h t h' t'. (h::t = h' :: t') = (h = h') /\ (t = t')          *)
+(*---------------------------------------------------------------------------*)
+
 val CONS_11 = save_thm("CONS_11", prove_constructors_one_one list_Axiom);
 
 val NOT_NIL_CONS = save_thm("NOT_NIL_CONS",
@@ -402,25 +458,25 @@ val NOT_CONS_NIL = save_thm("NOT_CONS_NIL",
    CONV_RULE(ONCE_DEPTH_CONV SYM_CONV) NOT_NIL_CONS);
 
 val LIST_NOT_EQ = store_thm("LIST_NOT_EQ",
- --`!l1 l2. ~(l1 = l2) ==> !h1:'a. !h2. ~(CONS h1 l1 = CONS h2 l2)`--,
+ --`!l1 l2. ~(l1 = l2) ==> !h1:'a. !h2. ~(h1::l1 = h2::l2)`--,
    REPEAT GEN_TAC THEN
    STRIP_TAC THEN
    ASM_REWRITE_TAC [CONS_11]);
 
 val NOT_EQ_LIST = store_thm("NOT_EQ_LIST",
- --`!h1:'a. !h2. ~(h1 = h2) ==> !l1 l2. ~(CONS h1 l1 = CONS h2 l2)`--,
+ --`!h1:'a. !h2. ~(h1 = h2) ==> !l1 l2. ~(h1::l1 = h2::l2)`--,
     REPEAT GEN_TAC THEN
     STRIP_TAC THEN
     ASM_REWRITE_TAC [CONS_11]);
 
 val EQ_LIST = store_thm("EQ_LIST",
- --`!h1:'a.!h2.(h1=h2) ==> !l1 l2. (l1 = l2) ==> (CONS h1 l1 = CONS h2 l2)`--,
+ --`!h1:'a.!h2.(h1=h2) ==> !l1 l2. (l1 = l2) ==> (h1::l1 = h2::l2)`--,
      REPEAT STRIP_TAC THEN
      ASM_REWRITE_TAC [CONS_11]);
 
 
 val CONS = store_thm   ("CONS",
-  --`!l : 'a list. ~NULL l ==> (CONS (HD l) (TL l) = l)`--,
+  --`!l : 'a list. ~NULL l ==> (HD l :: TL l = l)`--,
        STRIP_TAC THEN
        STRIP_ASSUME_TAC (SPEC (--`l:'a list`--) list_CASES) THEN
        POP_ASSUM SUBST1_TAC THEN
@@ -452,7 +508,7 @@ val LENGTH_MAP = store_thm ("LENGTH_MAP",
      LIST_INDUCT_TAC THEN ASM_REWRITE_TAC [MAP, LENGTH]);
 
 val EVERY_EL = store_thm ("EVERY_EL",
- --`!(l:'a list) P. EVERY P l = !n. (n < LENGTH l) ==> P (EL n l)`--,
+ --`!(l:'a list) P. EVERY P l = !n. n < LENGTH l ==> P (EL n l)`--,
       LIST_INDUCT_TAC THEN
       ASM_REWRITE_TAC [EVERY_DEF, LENGTH, NOT_LESS_0] THEN
       REPEAT STRIP_TAC THEN EQ_TAC THENL
@@ -474,7 +530,7 @@ val EVERY_CONJ = store_thm("EVERY_CONJ",
      FIRST_ASSUM ACCEPT_TAC);
 
 val LENGTH_NIL = store_thm("LENGTH_NIL",
- --`!l:'a list. (LENGTH l = 0) = (l = NIL)`--,
+ --`!l:'a list. (LENGTH l = 0) = (l = [])`--,
       LIST_INDUCT_TAC THEN
       REWRITE_TAC [LENGTH, NOT_SUC, NOT_CONS_NIL]);
 
@@ -517,7 +573,7 @@ val LENGTH_EQ_NIL = store_thm("LENGTH_EQ_NIL",
     [ASM_REWRITE_TAC [], ASM_REWRITE_TAC [LENGTH,NOT_SUC]]]);;
 
 val CONS_ACYCLIC = store_thm("CONS_ACYCLIC",
-Term`!l x. ~(l = CONS x l) /\ ~(CONS x l = l)`,
+Term`!l x. ~(l = x::l) /\ ~(x::l = l)`,
  LIST_INDUCT_TAC
  THEN ASM_REWRITE_TAC[CONS_11,NOT_NIL_CONS, NOT_CONS_NIL, LENGTH_NIL]);
 
@@ -553,7 +609,7 @@ val _ = adjoin_to_theory
   end)};
 
 val WF_LIST_PRED = store_thm("WF_LIST_PRED",
-Term`WF \L1 L2. ?h:'a. L2 = CONS h L1`,
+Term`WF \L1 L2. ?h:'a. L2 = h::L1`,
 REWRITE_TAC[relationTheory.WF_DEF] THEN BETA_TAC THEN GEN_TAC
   THEN CONV_TAC CONTRAPOS_CONV
   THEN Ho_rewrite.REWRITE_TAC
@@ -564,6 +620,132 @@ REWRITE_TAC[relationTheory.WF_DEF] THEN BETA_TAC THEN GEN_TAC
   THEN RULE_ASSUM_TAC(REWRITE_RULE[NOT_NIL_CONS,CONS_11])
   THENL [FIRST_ASSUM ACCEPT_TAC,
          PAT_ASSUM (Term`x /\ y`) (SUBST_ALL_TAC o CONJUNCT2) THEN RES_TAC]);
+
+(*---------------------------------------------------------------------------
+     Congruence rules for higher-order functions. Used when making
+     recursive definitions by so-called higher-order recursion.
+ ---------------------------------------------------------------------------*)
+
+val Induct = INDUCT_THEN list_INDUCT STRIP_ASSUME_TAC;
+
+val list_size_cong = store_thm("list_size_cong",
+Term
+  `!M N f f'. 
+    (M=N) /\ (!x. MEM x N ==> (f x = f' x))
+          ==>
+    (list_size f M = list_size f' N)`,
+Induct 
+  THEN REWRITE_TAC [list_size_def,MEM]
+  THEN REPEAT STRIP_TAC 
+  THEN PAT_ASSUM (Term`x = y`) (SUBST_ALL_TAC o SYM) 
+  THEN REWRITE_TAC [list_size_def]
+  THEN MK_COMB_TAC THENL
+  [NTAC 2 (MK_COMB_TAC THEN TRY REFL_TAC)
+     THEN FIRST_ASSUM MATCH_MP_TAC THEN REWRITE_TAC [MEM],
+   FIRST_ASSUM MATCH_MP_TAC THEN REWRITE_TAC [] THEN GEN_TAC
+     THEN PAT_ASSUM (Term`!x. MEM x l ==> Q x`) 
+                    (MP_TAC o SPEC (Term`x:'a`))
+     THEN REWRITE_TAC [MEM] THEN REPEAT STRIP_TAC
+     THEN FIRST_ASSUM MATCH_MP_TAC THEN ASM_REWRITE_TAC[]]);
+
+val FOLDR_CONG = store_thm("FOLDR_CONG",
+Term
+  `!l l' b b' (f:'a->'b->'b) f'. 
+    (l=l') /\ (b=b') /\ (!x a. MEM x l' ==> (f x a = f' x a))
+          ==>
+    (FOLDR f b l = FOLDR f' b' l')`,
+Induct 
+  THEN REWRITE_TAC [FOLDR,MEM]
+  THEN REPEAT STRIP_TAC 
+  THEN REPEAT (PAT_ASSUM (Term`x = y`) (SUBST_ALL_TAC o SYM))
+  THEN REWRITE_TAC [FOLDR]
+  THEN POP_ASSUM (fn th => MP_TAC (SPEC (Term`h`) th) THEN ASSUME_TAC th)
+  THEN REWRITE_TAC [MEM]
+  THEN DISCH_TAC
+  THEN MK_COMB_TAC
+  THENL [CONV_TAC FUN_EQ_CONV THEN ASM_REWRITE_TAC [],
+         FIRST_ASSUM MATCH_MP_TAC THEN ASM_REWRITE_TAC []
+           THEN REPEAT STRIP_TAC
+           THEN FIRST_ASSUM MATCH_MP_TAC
+           THEN ASM_REWRITE_TAC [MEM]]);
+
+val FOLDL_CONG = store_thm("FOLDL_CONG",
+Term
+  `!l l' b b' (f:'b->'a->'b) f'. 
+    (l=l') /\ (b=b') /\ (!x a. MEM x l' ==> (f a x = f' a x))
+          ==>
+    (FOLDL f b l = FOLDL f' b' l')`,
+Induct 
+  THEN REWRITE_TAC [FOLDL,MEM]
+  THEN REPEAT STRIP_TAC 
+  THEN REPEAT (PAT_ASSUM (Term`x = y`) (SUBST_ALL_TAC o SYM))
+  THEN REWRITE_TAC [FOLDL]
+  THEN FIRST_ASSUM MATCH_MP_TAC
+  THEN REWRITE_TAC[]
+  THEN CONJ_TAC
+  THENL [FIRST_ASSUM MATCH_MP_TAC THEN ASM_REWRITE_TAC [MEM],
+         REPEAT STRIP_TAC THEN FIRST_ASSUM MATCH_MP_TAC
+           THEN ASM_REWRITE_TAC [MEM]]);
+
+
+val MAP_CONG = store_thm("MAP_CONG",
+Term
+  `!l1 l2 f f'. 
+    (l1=l2) /\ (!x. MEM x l2 ==> (f x = f' x))
+          ==>
+    (MAP f l1 = MAP f' l2)`,
+Induct THEN REWRITE_TAC [MAP,MEM]
+  THEN REPEAT STRIP_TAC 
+  THEN REPEAT (PAT_ASSUM (Term`x = y`) (SUBST_ALL_TAC o SYM))
+  THEN REWRITE_TAC [MAP]
+  THEN MK_COMB_TAC
+  THENL [MK_COMB_TAC THEN TRY REFL_TAC 
+            THEN FIRST_ASSUM MATCH_MP_TAC
+            THEN REWRITE_TAC [MEM],
+         FIRST_ASSUM MATCH_MP_TAC
+             THEN REWRITE_TAC [] THEN REPEAT STRIP_TAC 
+             THEN FIRST_ASSUM MATCH_MP_TAC
+             THEN ASM_REWRITE_TAC [MEM]]);
+
+val EXISTS_CONG = store_thm("EXISTS_CONG",
+Term
+  `!l1 l2 P P'. 
+    (l1=l2) /\ (!x. MEM x l2 ==> (P x = P' x))
+          ==>
+    (EXISTS P l1 = EXISTS P' l2)`,
+Induct THEN REWRITE_TAC [EXISTS_DEF,MEM]
+  THEN REPEAT STRIP_TAC 
+  THEN REPEAT (PAT_ASSUM (Term`x = y`) (SUBST_ALL_TAC o SYM))
+  THENL [PAT_ASSUM (Term`EXISTS x y`) MP_TAC THEN REWRITE_TAC [EXISTS_DEF],
+         REWRITE_TAC [EXISTS_DEF]
+           THEN MK_COMB_TAC
+           THENL [MK_COMB_TAC THEN TRY REFL_TAC 
+                    THEN FIRST_ASSUM MATCH_MP_TAC
+                    THEN REWRITE_TAC [MEM],
+                  FIRST_ASSUM MATCH_MP_TAC
+                    THEN REWRITE_TAC [] THEN REPEAT STRIP_TAC 
+                    THEN FIRST_ASSUM MATCH_MP_TAC
+                    THEN ASM_REWRITE_TAC [MEM]]]);;
+
+
+val EVERY_CONG = store_thm("EVERY_CONG",
+Term
+  `!l1 l2 P P'. 
+    (l1=l2) /\ (!x. MEM x l2 ==> (P x = P' x))
+          ==>
+    (EVERY P l1 = EVERY P' l2)`,
+Induct THEN REWRITE_TAC [EVERY_DEF,MEM]
+  THEN REPEAT STRIP_TAC 
+  THEN REPEAT (PAT_ASSUM (Term`x = y`) (SUBST_ALL_TAC o SYM))
+  THEN REWRITE_TAC [EVERY_DEF]
+  THEN MK_COMB_TAC
+  THENL [MK_COMB_TAC THEN TRY REFL_TAC 
+           THEN FIRST_ASSUM MATCH_MP_TAC THEN REWRITE_TAC [MEM],
+         FIRST_ASSUM MATCH_MP_TAC
+           THEN REWRITE_TAC [] THEN REPEAT STRIP_TAC 
+           THEN FIRST_ASSUM MATCH_MP_TAC
+           THEN ASM_REWRITE_TAC [MEM]]);
+
 
 val _ = export_theory();
 
